\documentclass[12pt]{article}
\usepackage[backend=biber]{biblatex}
\usepackage{amsmath}
\usepackage{listings}
\usepackage{graphicx}
\usepackage{caption}
\usepackage{subcaption}
\usepackage{commath}
\usepackage{hyperref}
\usepackage{url}
\usepackage{xcolor}
\usepackage{textcomp}
\usepackage{dirtytalk}
\usepackage{listings}
\usepackage{wasysym}
\usepackage{float}


% Parameters for displaying code.
\lstset{language=C++}
\lstset{basicstyle=\ttfamily\small}
\lstset{frame=single}
\lstset{keywordstyle=\color{red}\bfseries}
\lstset{commentstyle=\itshape\color{blue}}
\lstset{showspaces=false}
\lstset{showstringspaces=false}
\lstset{showtabs=false}
\lstset{breaklines}

% Define new commands
\newcommand{\expect}[1]{\langle #1 \rangle}
\newcommand{\dd}[1]{\ \text{d}#1}
\newcommand{\f}[2]{\frac{#1}{#2}} 
\newcommand{\tf}[2]{\tfrac{#1}{#2}}
\newcommand{\beq}{\begin{equation*}}
\newcommand{\eeq}{\end{equation*}}
\newcommand{\bra}[1]{\langle #1|}
\newcommand{\ket}[1]{|#1 \rangle}
\newcommand{\braket}[2]{\langle #1 | #2 \rangle}
\newcommand{\av}[1]{\left| #1 \right|}
\newcommand{\op}[1]{\widehat{#1}}
\newcommand{\braopket}[3]{\langle #1 | \op{#2} | #3 \rangle}
\newcommand{\ketbra}[2]{\ket{#1}\bra{#2}}
\newcommand{\pp}[1]{\frac{\partial}{\partial #1}}
\newcommand{\ppn}[1]{\frac{\partial^2}{\partial #1^2}}
\newcommand{\up}{\left|\uparrow\rangle\right.}
\newcommand{\down}{\left|\downarrow\rangle\right.}
\newcommand{\updown}{\left|\uparrow\downarrow\rangle\right.}
\newcommand{\downup}{\left|\downarrow\uparrow\rangle\right.}
\newcommand{\ua}{\uparrow}
\newcommand{\da}{\downarrow}

% Add bibliography
%\addbibresource{bibliography.bib}

\begin{document}

\title{Derivations}
\author{Garbage}
\maketitle

\section*{Drift Force without interaction}

Drift force is given by:
\beq
F = \f{2\nabla\Psi_T}{\Psi_T}
\eeq
With non-interacting particles, we have
\beq
\Psi_T = \prod_{i} g(\alpha, \beta, \vec{r}_i)
\eeq
so
\begin{align*}
	\nabla g(\alpha, \beta, \vec{r}_i) &= 
	\left( \pp{x}+\pp{y}+\pp{z}\right)
	\exp\big(-\alpha(x^{2}_i + y^{2}_i + \beta z^{2}_i)\big)
\end{align*}
The partial derivatives are:
\begin{align*}
	\pp{x}g &= -2\alpha x_i \exp\big(-\alpha(x^{2}_i + y^{2}_i + \beta z^{2}_i)\big) \\
	\pp{y}g &= -2\alpha y_i \exp\big(-\alpha(x^{2}_i + y^{2}_i + \beta z^{2}_i)\big) \\
	\pp{z}g &= -2\alpha\beta z_i \exp\big(-\alpha(x^{2}_i + y^{2}_i) + \beta z^{2}_i)\big)
\end{align*}
Using this we find:
\begin{align*}
	\nabla g(\alpha, \beta, \vec{r}_i) &= 
	-2\alpha(x_i + y_i + \beta z_i)\exp\big(-\alpha(x^{2}_i + y^{2}_i) + \beta z^{2}_i)\big)
\end{align*}
Which finally gives:
\beq
	F = \f{2\nabla g}{g} = -4\alpha \sum_{i}(x_i + y_i + \beta z_i)
\eeq

\section{Local energy without interaction}
\subsection{Single particle}
\subsection{N particles}
\subsubsection{1D}
Edit 09.03.18: This is probably wrong. Check.
For N particles in one dimension, we have:
\begin{align*}
	\Psi_T &= \prod_{i} g(\alpha, \vec{r}_i) = \exp\big(-\alpha(x^{2}_i)\big) \\
	E_L &= \f{\op{H}\Psi_T}{\Psi_T} \\
	\op{H}\Psi_T &= \big(\sum_{i} \f{\hbar^2}{2m}\nabla^{2}_j + 
	\f{1}{2}m\omega^{2}_{ho}x^{2}_i \big) \prod_{i} g_i \\
	&= \f{\hbar^2}{2m}\sum_{i} \nabla^{2}_j \prod_{i} g_i + 
	\f{1}{2}m\omega^{2}_{ho}x^{2}_i \prod_{i} g_i \\
	\nabla^{2}_i &= \ppn{x_i}
\end{align*}
Computing the second-derivative of the wave-function:
\begin{align*}
	\nabla_j \prod_{i}g_i &=\pp{x_j}\prod_{i\neq j}g_i = -2\alpha x_i\prod_{i} g_i \\
	\nabla^{2}_j\prod_{i}g_i &= \nabla_j(\nabla_j \prod_{i}g_i) \\
	&= -2\alpha \nabla_j(x_i\prod_{i} g_i) \\
	&= -2\alpha \big(\prod_{i}g_i + x_i\nabla_j\prod_{i}g_i \big) \\
	&= -2\alpha \big(\prod_{i}g_i + x_i(-2\alpha x_i \prod_{i}g_)\big) \\
	&= 2\alpha\prod_{i}g_i(2\alpha x^{2}_i - 1)
\end{align*}
With this we find the local energy $E_L$:
\begin{align*}
	E_L &= 
	\f{1}{\prod_{i}g_i}\big(-\f{\hbar^2}{2m}\sum_{j}2\alpha\prod_{i}g_i
	(2\alpha x^{2}_i - 1) + \f{1}{2}m\omega^{2}_{ho}\prod_{i}g_i \big) \\
	&= -\f{\hbar^2}{m}\alpha N(2\alpha x^{2}_i - 2) + \f{1}{2}m\omega^{2}_{ho}
\end{align*}
where $\alpha = \f{1}{2a^{2}_{H_0}}$ and $a_{H_0} = \f{\hbar}{m\omega}$

\subsubsection{2D}
\subsubsection{3D}
Edited 08.03.18.
\begin{align*}
	\nabla_k\Psi_T(\vec{r}) &= \nabla_k\phi(\vec{r}_k)\cdot\prod_{i \neq k}\phi(\vec{r}_i) \\
	\nabla^{2}_{k}\Psi_T(\vec{r}) &=\nabla_k[\nabla_k\Psi_T(\vec{r})] \\
	&= \nabla_k[\nabla_k\phi(\vec{r}_k)\cdot\prod_{i \neq k}\phi(\vec{r}_i)] \\
	&= \nabla^{2}_{k}\phi(\vec{r}_k)\cdot\prod_{i \neq k}\phi(\vec{r}_i)\\
\end{align*}
where
\begin{align*}
	\nabla_k\phi(\vec{r}_k) &= \nabla_k\exp(-\alpha(x{^2}_k+y{^2}_k+\beta z{^2}_k)) \\
	&= -2\alpha(x_k + y_k + \beta z_k)\exp(-\alpha(x{^2}_k+y{^2}_k+\beta z{^2}_k))
\end{align*}
and
\begin{align*}
	\nabla^{2}_{k}\phi(\vec{r}_k) &= \nabla_k\big(\nabla_k
		\exp(-\alpha(x{^2}_k+y{^2}_k+\beta z{^2}_k))\big) \\
	&= \nabla_k\big(-2\alpha(x_k + y_k + \beta z_k)
		\exp(-\alpha(x{^2}_k+y{^2}_k+\beta z{^2}_k))\big) \\
	&= -2\alpha\big(\nabla_k(x_k + y_k + \beta z_k)
		\cdot\exp(-\alpha(x{^2}_k+y{^2}_k+\beta z{^2}_k)) \\
		&+ \nabla_k\exp(-\alpha(x{^2}_k+y{^2}_k+\beta z{^2}_k))
		\cdot(x_k + y_k + \beta z_k)\big) \\
	&= -2\alpha\big(\nabla_k(x_k + y_k + \beta z_k)\cdot\phi(\vec{r}_k)
		-2\alpha(x_k + y_k + \beta z_k)^2\phi(\vec{r}_k)\big) \\
	&= -2\alpha\big((2+\beta)\phi(\vec{r}_k)
		-2\alpha(x_k + y_k + \beta z_k)^2\phi(\vec{r}_k)\big) \\
\end{align*}

\section{Local energy with interaction}
\subsection{Note on indices in project file.}
The project file has screwed up indices for sums etc in the problem text,
and lacks some clarity regarding $f(i,j)$. This is a brief summary of notes made
in group session:
\begin{align*}
	\phi{\vec{r}_i} &= \exp(-\alpha(x^{2}_i + y^{2}_i + \beta z^{2}_i))\\
	f(r_{ij}) &= \exp(\sum_{i<j}u(r_{ij})) \\
	u(r_{ij}) &= ln(f(r_{ij})) = ln(\exp\big(\sum_{i<j}u(r_{ij})\big)) \\
	f(r_{ij}) &= \exp\big(u(r_{ij})\big) \\
	\nabla_k \exp\big(\sum_{i<j} u(r_{ij}) &= \exp\big(\sum_{i<j} u(r_{ij})\big) \cdot 
	\nabla_k \sum_{l\neq k} u(r_{lk}) \\
	\sum_{j\neq k} \nabla_k u(r_{kj})
\end{align*}


\end{document}
